Core/Ty/Definition.lean
@@ -1,5 +1,7 @@
+
 inductive BaseKind : Type where
-| «open» | closed
+| closed
+| «open»
 
 inductive Kind : Type where
 | base : BaseKind -> Kind
@@ -12,36 +14,36 @@ infixr:64 " -:> " => Kind.arrow
 inductive Ty : Type where
 | var : Nat -> Ty
 | global : String -> Ty
-| arrow : Ty -> Ty -> Ty
+| arrow : BaseKind -> Ty -> Ty -> Ty
 | all : Kind -> Ty -> Ty
 | app : Ty -> Ty -> Ty
 | eq : Kind -> Ty -> Ty -> Ty
 
 prefix:max "t#" => Ty.var
 prefix:max "gt#" => Ty.global
-infixr:64 " -:> " => Ty.arrow
+notation A:64 " -[" b "]>" B:65 => Ty.arrow b A B
+infixr:64 " -:> " => Ty.arrow BaseKind.closed
+infixr:64 " =:> " => Ty.arrow BaseKind.open
 notation "∀[" K "]" B => Ty.all K B
 infixl:54 " • " => Ty.app
 notation:55 A:55 " ~[" K "]~ " B => Ty.eq K A B
 
 protected def Kind.repr (p : Nat) : (a : Kind) -> Std.Format
-| .base .closed => "★"
-| .base .open => "◯"
-| .arrow k1 k2 => Repr.addAppParen ((Kind.repr max_prec k1) ++ " -:> " ++ Kind.repr p k2) p
+| base .closed => "★"
+| base .open => "◯"
+| arrow k1 k2 => Repr.addAppParen ((Kind.repr max_prec k1) ++ " -:> " ++ Kind.repr p k2) p
 
 instance kindRepr : Repr Kind where
   reprPrec a p := Kind.repr p a
 
 protected def Ty.repr (p : Nat) : (a : Ty) -> Std.Format
-| .var n => "t#" ++ Nat.repr n
-| .global s => "gt#" ++ s
-| .arrow t1 t2 => Repr.addAppParen (Ty.repr max_prec t1 ++ " -:> " ++ Ty.repr p t2) p
-| .all K t => Repr.addAppParen ("∀[ " ++ repr K ++ " ] " ++ Ty.repr max_prec t) p
-| .eq K A B => Repr.addAppParen (Ty.repr max_prec A ++ " ~[" ++ repr K ++ "]~ " ++ Ty.repr max_prec B) p
-| .app t1 t2 => Repr.addAppParen (Ty.repr p t1 ++ " • " ++ Ty.repr max_prec t2) p
+| var n => "t#" ++ Nat.repr n
+| global s => "gt#" ++ s
+| arrow .closed t1 t2 => Repr.addAppParen (Ty.repr max_prec t1 ++ " -:> " ++ Ty.repr p t2) p
+| arrow .open t1 t2 => Repr.addAppParen (Ty.repr max_prec t1 ++ " =:> " ++ Ty.repr p t2) p
+| all K t => Repr.addAppParen ("∀[ " ++ repr K ++ " ] " ++ Ty.repr max_prec t) p
+| eq K A B => Repr.addAppParen (Ty.repr max_prec A ++ " ~[" ++ repr K ++ "]~ " ++ Ty.repr max_prec B) p
+| app t1 t2 => Repr.addAppParen (Ty.repr p t1 ++ " • " ++ Ty.repr max_prec t2) p
 
 instance tyRepr : Repr Ty where
   reprPrec a p := Ty.repr p a
-
-
-#eval (∀[ (★ -:> ★) -:> ★] t#0 -:> (gt#"Eq" • (t#0 • gt#"Bool")))
