Core/Global.lean
@@ -9,29 +9,71 @@ inductive Global : Type where
 | data : String -> Kind -> Vec (String × Ty) n -> Global
 | opent : String -> Kind -> Global
 | openm : String -> Ty -> Global
-| «let» : String -> Ty -> Term -> Global
+| defn : String -> Ty -> Term -> Global
 | inst : String -> Term -> Global
 | instty : String -> Ty -> Global
 
-def lookup_kind (x : String) : List Global -> Option Kind
-| [] => none
-| .cons (.data n K _) t
-| .cons (.opent n K) t =>
-  if n == x then K else lookup_kind x t
-| .cons _ t => lookup_kind x t
+inductive Entry : Type where
+| data : String -> Kind -> Entry
+| ctor : String -> Nat -> Ty -> Entry
+| opent : String -> Kind -> Entry
+| openm : String -> Ty -> Entry
+| defn : String -> Ty -> Term -> Entry
+| instty : String -> Ty -> Entry
 
-def lookup_type (x : String) : List Global -> Option Ty
+def Entry.is_data : Entry -> Bool
+| data _ _ => true
+| _ => false
+
+def Entry.is_ctor : Entry -> Bool
+| ctor _ _ _ => true
+| _ => false
+
+def Entry.is_opent : Entry -> Bool
+| opent _ _ => true
+| _ => false
+
+def Entry.is_openm : Entry -> Bool
+| openm _ _ => true
+| _ => false
+
+def Entry.is_defn : Entry -> Bool
+| defn _ _ _ => true
+| _ => false
+
+def Entry.is_instty : Entry -> Bool
+| instty _ _ => true
+| _ => false
+
+def Entry.kind : Entry -> Option Kind
+| data _ K => K
+| opent _ K => K
+| _ => none
+
+def Entry.type : Entry -> Option Ty
+| ctor _ _ T => T
+| openm _ T => T
+| defn _ T _ => T
+| instty _ T => T
+| _ => none
+
+def lookup (x : String) : List Global -> Option Entry
 | [] => none
-| .cons (.data (n := n) _ _ ctors) t =>
-  let ctors : Vec (Option Ty) n := λ i =>
-    let (y, A) := ctors i
-    if y == x then A else none
-  Vec.fold Option.or (lookup_type x t) ctors
-| .cons (.openm n A) t
-| .cons (.let n A _) t
-| .cons (.instty n A) t =>
-  if n == x then A else lookup_type x t
-| .cons _ t => lookup_type x t
+| .cons (.data (n := n) y K ctors) tl =>
+  let ctors : Vec (Option Entry) n := λ i =>
+    let (z, A) := ctors i
+    if x == z then return .ctor z i A else none
+  if x == y then return .data y K
+  else Vec.fold Option.or (lookup x tl) ctors
+| .cons (.opent y a) tl =>
+  if x == y then return .opent y a else lookup x tl
+| .cons (.openm y a) tl =>
+  if x == y then return .openm y a else lookup x tl
+| .cons (.defn y a b) tl =>
+  if x == y then return .defn y a b else lookup x tl
+| .cons (.inst _ _) tl => lookup x tl
+| .cons (.instty y a) tl =>
+  if x == y then return .instty y a else lookup x tl
 
 def instances (x : String) : List Global -> List Term
 | [] => []
@@ -39,16 +81,18 @@ def instances (x : String) : List Global -> List Term
   if x == y then t :: instances x tl else instances x tl
 | .cons _ tl => instances x tl
 
-def is_ctor : List Global -> String -> Bool := sorry
+def lookup_kind G x := lookup x G |> Option.map Entry.kind |> Option.get!
+def lookup_type G x := lookup x G |> Option.map Entry.type |> Option.get!
+def is_ctor G x := lookup x G |> Option.map Entry.is_ctor |> Option.get!
+def is_data G x := lookup x G |> Option.map Entry.is_data |> Option.get!
+def is_instty G x := lookup x G |> Option.map Entry.is_instty |> Option.get!
+def is_opent G x := lookup x G |> Option.map Entry.is_opent |> Option.get!
+def is_openm G x := lookup x G |> Option.map Entry.is_openm |> Option.get!
 
-def is_datatype : List Global -> String -> Bool := sorry
+def ctor_idx (x : String) (G : List Global) : Option Nat := do
+  let t <- lookup x G
+  match t with
+  | .ctor _ n _ => n
+  | _ => none
 
-def is_instty : List Global -> String -> Bool := sorry
-
-def is_opent : List Global -> String -> Bool := sorry
-
-def is_openm : List Global -> String -> Bool := sorry
-
-def ctor_idx : List Global -> String -> Option (Fin n) := sorry
-
-def is_stable : List Global -> String -> Bool := sorry
+def is_stable (x : String) (G : List Global) : Bool := !is_openm G x
