Core/Reduction/Congr.lean
@@ -1,0 +1,55 @@
+import Core.Reduction.Definition
+
+-- Ctor2 Congr1
+@[simp]
+theorem Ctor2Variant.congr1_app : congr1 (app b) = true := by simp [congr1]
+
+@[simp]
+theorem Ctor2Variant.congr1_cast : congr1 cast = false := by simp [congr1]
+
+@[simp]
+theorem Ctor2Variant.congr1_seq : congr1 seq = true := by simp [congr1]
+
+@[simp]
+theorem Ctor2Variant.congr1_appc : congr1 appc = true := by simp [congr1]
+
+@[simp]
+theorem Ctor2Variant.congr1_apptc : congr1 apptc = true := by simp [congr1]
+
+@[simp]
+theorem Ctor2Variant.congr1_arrowc : congr1 arrowc = true := by simp [congr1]
+
+@[simp]
+theorem Ctor2Variant.congr1_choice : congr1 choice = true := by simp [congr1]
+
+-- Ctor2 Congr2
+@[simp]
+theorem Ctor2Variant.congr2_app : congr2 (app .closed) = false := by simp [congr2]
+
+@[simp]
+theorem Ctor2Variant.congr2_appo : congr2 (app .open) = true := by simp [congr2]
+
+@[simp]
+theorem Ctor2Variant.congr2_cast : congr2 cast = true := by simp [congr2]
+
+@[simp]
+theorem Ctor2Variant.congr2_seq : congr2 seq = true := by simp [congr2]
+
+@[simp]
+theorem Ctor2Variant.congr2_appc : congr2 appc = true := by simp [congr2]
+
+@[simp]
+theorem Ctor2Variant.congr2_apptc : congr2 apptc = true := by simp [congr2]
+
+@[simp]
+theorem Ctor2Variant.congr2_arrowc : congr2 arrowc = true := by simp [congr2]
+
+@[simp]
+theorem Ctor2Variant.congr2_choice : congr2 choice = true := by simp [congr2]
+
+-- TyBind Congr
+@[simp]
+theorem TyBindVariant.congr_lamt : congr lamt = false := by simp [congr]
+
+@[simp]
+theorem TyBindVariant.congr_allc : congr allc = true := by simp [congr]
