Core/Reduction/Value.lean
@@ -1,0 +1,50 @@
+import LeanSubst
+import Core.Term
+import Core.Reduction.Definition
+import Core.Reduction.Congr
+
+open LeanSubst
+
+@[simp]
+theorem Value.not_zero : ¬ Value G `0 := by
+  intro j; cases j
+  case _ x sp j1 j2 j3 =>
+  simp [Term.spine] at j3
+
+theorem Value.sound : Value G t -> ∀ t', ¬ (G ⊢ t ~> t') := by
+  intro j; induction j <;> intro t' r
+  case app x sp t j1 j2 j3 ih =>
+    cases t
+    all_goals try simp [Term.spine] at j1
+    case global y =>
+      rcases j1 with ⟨e1, e2⟩; subst e1 e2
+      cases r; case _ z sp T tl tl' q1 q2 q3 q4 q5 q6 q7 q8 =>
+      simp [Term.spine] at q7
+      rcases q7 with ⟨e1, e2⟩; subst e1 e2; simp at *
+      cases j3
+      case _ j3 =>
+
+        sorry
+      case _ j3 =>
+        sorry
+    case ctor1 c t =>
+      cases c <;> simp [Term.spine] at j1
+      case appt =>
+        sorry
+    case ctor2 c t1 t2 =>
+      cases c <;> try simp [Term.spine] at j1
+      case app => sorry
+      -- case appo =>
+      --   replace j1 := Eq.symm j1
+      --   rw [Option.bind_eq_some_iff] at j1
+      --   rcases j1 with ⟨q, e1, e2⟩
+      --   rcases q with ⟨y, sp'⟩; simp at e2
+      --   rcases e2 with ⟨e2, e3⟩; subst e2 e3
+      --   sorry
+  case choice t1 t2 j1 j2 ih1 ih2 =>
+    cases r <;> simp at *
+    case inst h _ _ => simp [Term.spine] at h
+    case ctor2_congr1 r _ => apply ih1 _ r
+    case ctor2_congr2 r _ => apply ih2 _ r
+  all_goals
+    cases r <;> simp [Term.spine] at *
