Core/Ty/BEq.lean
@@ -1,8 +1,8 @@
 import Core.Ty.Definition
 
 def BaseKind.beq : BaseKind -> BaseKind -> Bool
-| .open, .open => true
 | closed, closed => true
+| .open, .open => true
 | _, _ => false
 
 instance : BEq BaseKind where
@@ -19,7 +19,7 @@ instance : BEq Kind where
 def Ty.beq : Ty -> Ty -> Bool
 | var x, var y => x == y
 | global x, global y => x == y
-| arrow A1 B1, arrow A2 B2 => beq A1 A2 && beq B1 B2
+| arrow b1 A1 B1, arrow b2 A2 B2 => b1 == b2 && beq A1 A2 && beq B1 B2
 | all K1 P1, all K2 P2 => K1 == K2 && beq P1 P2
 | app A1 B1, app A2 B2 => beq A1 A2 && beq B1 B2
 | eq K1 A1 B1, eq K2 A2 B2 => K1 == K2 && beq A1 A2 && beq B1 B2
